scripts/hol-probes/regenerate.sh
@@ -604,7 +604,7 @@ run_probe compile_to_crep_probeScript.sml compile_to_crep_probe.out \
   empty raise_const raise_pair raise_pair_later raise_pair_later_64 handled_pair done \
   "$cake_dir/pancake/pan_to_crepScript.sml"
 run_probe crep_alookup_compile_probeScript.sml crep_alookup_compile_probe.out \
-  alookup_empty_params alookup_param_entry "$cake_dir/pancake/pan_to_crepScript.sml"
+  source_names_distinct alookup_param_entry "$cake_dir/pancake/pan_to_crepScript.sml"
 run_probe dup_exn_eids_probeScript.sml dup_exn_eids_probe.out \
   dup_eids_lookup mixed_eids_lookup_a mixed_eids_lookup_e dup_compile done \
   "$cake_dir/pancake/pan_to_crepScript.sml"
